\documentclass[12pt]{article}

\usepackage[margin=1in]{geometry}
\usepackage{fancyhdr}
\usepackage{setspace}
\pagestyle{fancy}
\usepackage{amsmath, amsthm, amssymb, amsfonts, mathtools, xfrac,mathrsfs}
\usepackage[utf8]{inputenc}
\usepackage[english]{babel}
\usepackage{graphicx,dsfont}
\usepackage{braket, bm}
\usepackage[dvipsnames]{xcolor}

\everymath{\displaystyle}
\headheight=20pt

\usepackage{listings}
\lstset{frame=single,
  language=Python,
  showstringspaces=false,
  columns=flexible,
  basicstyle={\small\ttfamily},
  keywordstyle=\bfseries\color{OliveGreen},
  commentstyle=\itshape\color{purple},
  identifierstyle=\color{blue},
  stringstyle=\color{red},
  numbers=none,
  breaklines=true,
  breakatwhitespace=true
  tabsize=3
}

\newcommand{\N}{\mathbb{N}}

\newenvironment{problem}[2][Problem]{\begin{trivlist}
\item[\hskip \labelsep {\bfseries #1}\hskip \labelsep {\bfseries #2.}]}{\end{trivlist}}


\title{Homework}
\lhead{DSGE Models}
\chead{Pset 4}
\rhead{Alex Weinberg}

%-------------------------------------------------------------------------------

\begin{document}

\begin{problem}{1}
For this case find an algebraic solution for the policy function, $k_{t+1} = \phi(k_t,z_t)$.
\begin{proof}
 We first guess, that there exists $A$ defining the policy function $K_{t+1} = Ae^{zt}K_t^\alpha$ and plugging it into the Euler equation. This gives us:
\begin{align*}
\frac{1}{ e^{z_t} K_t^\alpha - K_{t+1}} &= \beta E_t \big\{\frac{\alpha e^{z_{t+1}} K_{t+1}^{\alpha-1}}{e^{z_{t+1}}K_{t+1}^\alpha - K_{t+2}}\big\} \\
\frac{1}{ (1-A)e^{z_t} K_t^\alpha} &= \beta E_t \big\{\frac{\alpha e^{z_{t+1}} K_{t+1}^{\alpha-1}}{(1-A)e^{z_{t+1}}K_{t+1}^\alpha}\big\} \\
\frac{1}{ e^{z_t} K_t^\alpha} &= \beta \frac{\alpha}{K_{t+1}}\\
\frac{1}{ e^{z_t} K_t^\alpha} &= \beta \frac{\alpha}{Ae^{zt}K_t^\alpha}\\
1 &= \frac{\alpha \beta}{A}\\
A &= \alpha\beta
\end{align*}
\end{proof}
\end{problem}

%-------------------------------------------------------------------------------

\begin{problem}{2}
Given following functional forms,
\begin{equation}
\begin{split}
u(c_t,\ell_t) & = \text{ln }c_t + a \text{ ln }(1-\ell_t)\\
F(K_t,L_t,z_t) & = e^{z_t}K^{\alpha}_t L^{1-\alpha}_t  \nonumber
\end{split}
\end{equation} find the characterizing equations.
\begin{proof}
$$c_t = (1-\tau)(w_tl_t + (r_t -\delta)k_t) + k_t + T_t - k_{t+1}$$
$$\frac{1}{c_t} = \beta E_t \big\{ \frac{1}{c_{t+1}}((r_{t+1} - \delta)(1-\tau)+ 1) \big\}$$
$$\frac{a}{1-l_t} = \frac{w_t}{c_t}(1-\tau)$$
$$r_t = \alpha e^{zt}K_t^{\alpha-1} L_t^{1-\alpha}$$
$$w_t = (1-\alpha) e^{zt}K_t^{\alpha} L_t^{-\alpha}$$
$$\tau(w_tl_t + (r_t -\delta)k_t) = T_t$$
$$z_t = (1-p_z)\bar{z} + p_zz_{t-1} + \epsilon^z_t,  \epsilon^z_t \sim \text{i.i.d}(0, \sigma^2_z)$$
\end{proof}
\end{problem}

%-------------------------------------------------------------------------------

\begin{problem}{3}
Using CRRA utility for consumption,
\begin{equation}\label{DSGE_HW_CharEq_CES_Ln_eq01}
\begin{split}
u(c_t,\ell_t) & = \frac{c^{1-\gamma}_t -1}{1-\gamma}+ a \text{ ln }(1-\ell_t)\\
F(K_t,L_t,z_t) & = e^{z_t}K^{\alpha}_t L^{1-\alpha}_t  \nonumber
\end{split}
\end{equation}
\begin{proof}
New characterizing equations are similar
$$c_t = (1-\tau)(w_tl_t + (r_t -\delta)k_t) + k_t + T_t - k_{t+1}$$
$$\frac{1}{c_t^{-\gamma}} = \beta E_t \big\{ \frac{1}{c_{t+1}^{-\gamma}}((r_{t+1} - \delta)(1-\tau)+ 1) \big\}$$
$$\frac{a}{1-l_t} = \frac{w_t}{c_t^{-\gamma}}(1-\tau)$$
$$r_t = \alpha e^{zt}K_t^{\alpha-1} L_t^{1-\alpha}$$
$$w_t = (1-\alpha) e^{zt}K_t^{\alpha} L_t^{-\alpha}$$
$$\tau(w_tl_t + (r_t -\delta)k_t) = T_t$$
$$z_t = (1-p_z)\bar{z} + p_zz_{t-1} + \epsilon^z_t,  \epsilon^z_t \sim \text{i.i.d}(0, \sigma^2_z)$$
\end{proof}
\end{problem}

%-------------------------------------------------------------------------------

\begin{problem}{4}
Using CRRA utility for consumption and leisure and a new production function.
\begin{equation}\label{DSGE_HW_CharEq_CES_eq01}
\begin{split}
u(c_t,\ell_t) & = \frac{c^{1-\gamma}_t -1}{1-\gamma}+ a \frac{(1-\ell_t)^{1-\xi}-1}{1-\xi}      \\
F(K_t,L_t,z_t) & = e^{z_t}\left[\alpha K^{\eta}_t +(1-\alpha)L^{\eta}_t \right]^{\frac{1}{\eta}}   \nonumber
\end{split}
\end{equation}
\begin{proof}
New characterizing equations are similar
$$c_t = (1-\tau)(w_tl_t + (r_t -\delta)k_t) + k_t + T_t - k_{t+1}$$
$$\frac{1}{c_t^{-\gamma}} = \beta E_t \big\{ \frac{1}{c_{t+1}^{-\gamma}}((r_{t+1} - \delta)(1-\tau)+ 1) \big\}$$
$$\frac{a}{(1-l_t)^{-\xi}} = \frac{w_t}{c_t^{-\gamma}}(1-\tau)$$
$$r_t = \alpha e^{zt}K_t^{\eta-1} (\alpha K_t^\eta+ (1-\alpha)L_t^\eta)^{\frac{1-\eta}{\eta}}$$
$$w_t = (1-\alpha) e^{zt}L_t^{\eta-1}(\alpha K_t^\eta+ (1-\alpha)L_t^\eta)^{\frac{1-\eta}{\eta}}$$
$$\tau(w_tl_t + (r_t -\delta)k_t) = T_t$$
$$z_t = (1-p_z)\bar{z} + p_zz_{t-1} + \epsilon^z_t,  \epsilon^z_t \sim \text{i.i.d}(0, \sigma^2_z)$$
\end{proof}
\end{problem}

%-------------------------------------------------------------------------------

\begin{problem}{5}
Using the new given functional forms. Write out characterizing equations.
\begin{equation}\label{DSGE_HW_NoLeisure_eq01}
\begin{split}
u(c_t) & = \frac{c^{1-\gamma}_t -1}{1-\gamma}      \\
F(K_t,L_t,z_t) & = K^{\alpha}_t (L_te^{z_t})^{1-\alpha}  \nonumber
\end{split}
\end{equation}
We have 6 because intratemporal labor/leisure euler equation drops out.
\begin{proof}
\begin{align*}
c_t &= (1-\tau)(w_t+ (r_t -\delta)k_t) + k_t + T_t - k_{t+1} \\
\frac{1}{c_t^{-\gamma}} &= \beta E_t \big\{ \frac{1}{c_{t+1}^{-\gamma}}((r_{t+1} - \delta)(1-\tau)+ 1) \big\} \\
r_t &= \alpha (e^{zt})^{(1-\alpha)} K_t^{\alpha-1} \\
w_t &= (1-\alpha) (e^{zt})^{(1-\alpha)} K_t^{\alpha} \\
\tau(w_t + (r_t -\delta)k_t) &= T_t \\
z_t &= (1-p_z)\bar{z} + p_zz_{t-1} + \epsilon^z_t,  \epsilon^z_t \sim \text{i.i.d}(0, \sigma^2_z)
\end{align*}
In the non-stochastic steady state this becomes:
$$\bar{c} = (1-\tau)(\bar{w} + (\bar{r} -\delta)\bar{k}) + \bar{T}$$
$$\frac{1}{\bar{c}^{-\gamma}} = \beta \frac{1}{\bar{c}^{-\gamma}}((\bar{r} - \delta)(1-\tau)+ 1) $$
$$\bar{r} = \alpha (e^{\bar{z}})^{1-\alpha} \bar{k}^{\alpha-1} $$
$$\bar{w} = (1-\alpha) (e^{\bar{z}})^{1-\alpha} \bar{k}^{\alpha} $$
$$\tau(\bar{w} + (\bar{r} -\delta)\bar{k}) =  \bar{T}$$
With $\bar{z} = 0$. Solving algebraically for the steady state values of capital, output, and investment, giving us:
$$\bar{r} = \frac{\frac{1}{\beta}-1}{1-\tau} + \delta = 0.12$$
$$\bar{k} = \big(\frac{\bar{r}}{\alpha}\big)^\frac{1}{\alpha-1} = 7.28$$
$$\bar{I} = \delta \bar{k} = 0.73$$
$$\bar{Y} = \bar{k}^\alpha = 2.21$$
Numerical solution is similar. See jupyter notebook attached below.
\end{proof}
\end{problem}

%-------------------------------------------------------------------------------

\begin{problem}{6}
Using the new given functional forms,
\begin{equation}
\begin{split}
u(c_t,\ell_t) & = \frac{c^{1-\gamma}_t -1}{1-\gamma}+ a \frac{(1-\ell_t)^{1-\xi}-1}{1-\xi}      \\
F(K_t,L_t,z_t) & = K^{\alpha}_t (L_te^{z_t})^{1-\alpha}  \nonumber
\end{split}
\end{equation}
\begin{proof}
We have similar characterizing equations:
$$c_t = (1-\tau)(w_t+ (r_t -\delta)k_t) + k_t + T_t - k_{t+1}$$
$$\frac{1}{c_t^{-\gamma}} = \beta E_t \big\{ \frac{1}{c_{t+1}^{-\gamma}}((r_{t+1} - \delta)(1-\tau)+ 1) \big\}$$
$$\frac{a}{(1-l_t)^{-\xi}} = \frac{w_t}{c_t^{-\gamma}}(1-\tau)$$
$$r_t = \alpha (e^{zt})^{1-\alpha} K_t^{\alpha-1} L_t^ {1-\alpha}$$
$$w_t = (1-\alpha) (e^{zt})^{1-\alpha} K_t^{\alpha}L_t^ {-\alpha} $$
$$\tau(w_t + (r_t -\delta)k_t) = T_t$$
$$z_t = (1-p_z)\bar{z} + p_zz_{t-1} + \epsilon^z_t,  \epsilon^z_t \sim \text{i.i.d}(0, \sigma^2_z)$$
which in the steady state become:
$$\bar{c} = (1-\tau)(\bar{w} + (\bar{r} -\delta)\bar{k}) + \bar{T}$$
$$\frac{1}{\bar{c}^{-\gamma}} = \beta \frac{1}{\bar{c}^{-\gamma}}((\bar{r} - \delta)(1-\tau)+ 1) $$
$$\frac{a}{(1-\bar{l})^{-\xi}} = \frac{\bar{w}}{\bar{c}^{-\gamma}}(1-\tau)$$
$$\bar{r} = \alpha (e^{\bar{z}})^{1-\alpha} \bar{k}^{\alpha-1} \bar{l}^{1-\alpha} $$
$$\bar{w} = (1-\alpha) (e^{\bar{z}})^{1-\alpha} \bar{k}^{\alpha} \bar{l}^{-\alpha}$$
$$\tau(\bar{w} + (\bar{r} -\delta)\bar{k}) =  \bar{T}$$
where $\bar{z} = 0$.
Numerical solution is similar. See jupyter notebook attached below.
\end{proof}
\end{problem}


\end{document}
